Salt.v
@@ -33,7 +33,7 @@ Inductive instr : Type :=
   | sfree : nat -> instr
   | malloc : register -> nat -> instr
   | mov : register -> operand -> instr
-  | load : register -> register -> nat -> instr
+  | load : register -> register -> bool -> nat -> instr
   | store : register -> nat -> operand -> instr
   | push : operand -> instr
   | pop : register -> instr
@@ -52,9 +52,12 @@ Definition heap_val := (stack_heap_val + tuple_heap_val)%type.
 Inductive instr_seq : Type :=
   | ins_seq : list instr -> instr_seq.
 Definition reg_file : Type := list (register * word).
-Definition stack_heap : Type := list (heap_loc * stack_heap_val).
+Definition stack_heap : Type :=
+  list (heap_loc * stack_heap_val).
 Definition tuple_heap : Type := heap_loc -> tuple_heap_val.
-Definition heap : Type := (stack_heap * tuple_heap).
+(* K and E, continuations in heap, then tuples *)
+Definition heap : Type :=
+  (stack_heap * stack_heap * tuple_heap).
 Definition program : Type := code_loc -> instr_seq.
 
 (* Coercions *)
@@ -84,7 +87,8 @@ Definition reg_eqb a b :=
   | _,_ => false
   end.
 (* register file is always an ordered list *)
-Fixpoint reg_update (rf : reg_file) (x : register) (v : word) :=
+Fixpoint reg_update (rf : reg_file) (x : register)
+  (v : word) :=
   match x,rf with
   | _,nil => (x,v) :: nil
   | ip, (ip,w) :: rf' => (ip,v) :: rf'
@@ -111,7 +115,7 @@ Definition h_eqb a b :=
   end.
 Definition sh_empty : stack_heap := nil.
 Definition th_empty : tuple_heap := fun _ => tuple nil.
-Definition h_empty : heap := (sh_empty, th_empty).
+Definition h_empty : heap := (sh_empty, sh_empty, th_empty).
 Fixpoint sh_update (sh:stack_heap) (x:heap_loc)
   (v:stack_heap_val) :=
   match sh with
@@ -122,7 +126,8 @@ Fixpoint sh_update (sh:stack_heap) (x:heap_loc)
 Definition th_update (th:tuple_heap) (x:heap_loc)
   (v:tuple_heap_val) :=
   (fun x' => if h_eqb x x' then v else th x').
-Definition h_update (h : heap) (x : heap_loc) (v : heap_val) :=
+(*Definition h_update (h : heap) (x : heap_loc) 
+  (v : heap_val) :=
   match v, h with
   | inl (stack lst), (s_h,t_h) =>
     (sh_update s_h x (stack lst),t_h)
@@ -131,21 +136,25 @@ Definition h_update (h : heap) (x : heap_loc) (v : heap_val) :=
   (* undefined below *)
   | inl no_stacks, (s_h,t_h) => (s_h,t_h)
   end.
+Notation "x '!->h' v ';' m" := (h_update m x v)
+  (at level 100, v at next level, right associativity).*)
 Notation "x '!->s' v ';' m" := (sh_update m x v)
   (at level 100, v at next level, right associativity).
 Notation "x '!->t' v ';' m" := (th_update m x v)
   (at level 100, v at next level, right associativity).
-Notation "x '!->h' v ';' m" := (h_update m x v)
-  (at level 100, v at next level, right associativity).
+
 Definition c_eqb a b :=
   match a,b with
   | cloc_str a', cloc_str b' => eqb a' b'
   end.
-Definition c_update (m : program) (x : code_loc) (v : instr_seq) :=
+Definition c_update (m : program) (x : code_loc)
+  (v : instr_seq) :=
   fun x' => if c_eqb x x' then v else m x'.
-(* Fixpoint (*code_fetch*) (c: program) (lab: code_loc) : instr_seq :=
+(* Fixpoint (*code_fetch*) (c: program) (lab: code_loc)
+ : instr_seq :=
   match c with
-  | cons (x,v) c' => if c_eqb x lab then v else (*code_fetch*) c' lab
+  | cons (x,v) c' => if c_eqb x lab then v else 
+    (*code_fetch*) c' lab
   | nil => empty_seq
   end.
 *)
@@ -215,24 +224,48 @@ Definition operand_value o (r_file:reg_file) :=
    -------------------------------------------- *)
 Fixpoint stk_heap_app (sh: stack_heap) (loc: heap_loc) :=
   match sh with
-  | (x,v) :: sh' => if h_eqb x loc then v else stk_heap_app sh' loc
+  | (x,v) :: sh' =>
+    if h_eqb x loc then v else stk_heap_app sh' loc
   | [] => no_stacks
   end.
-
-(* returns word at given heap memory address *)
+Definition fresh (h:heap) (loc:heap_loc) : bool :=
+  match h with (s1,s2,t) =>
+    match stk_heap_app s1 loc, stk_heap_app s2 loc, t loc with
+    | no_stacks, no_stacks, tuple nil => true
+    | _,_,_ => false
+    end
+  end.
+(* returns word at given heap memory address
 Definition heap_app (h: heap) (loc:heap_loc) :=
   match h with (s_h,t_h) =>
     match stk_heap_app s_h loc with
     | stack lst => inl (stack lst)
     | no_stacks => inr (t_h loc)
     end
+  end.*)
+(* Definition fetch_heap (loc:heap_loc) (i:nat) (h:heap) :=
+  match h with (s_h1,s_h2,t_h) =>
+    match stk_heap_app s_h1 loc,
+      stk_heap_app s_h2 loc,t_h loc with
+    | stack lst,no_stacks,tuple [] =>
+      nth ((List.length lst)-i) lst ns
+    | no_stacks,stack lst,tuple [] =>
+      nth ((List.length lst)-i) lst ns
+    | no_stacks,no_stacks,tuple lst => nth i lst ns
+    | _,_,_ => ns
+    end
   end.
+*)
 Definition fetch_heap (loc:heap_loc) (i:nat) (h:heap) :=
-  match h with (s_h,t_h) =>
-    match stk_heap_app s_h loc with
-    | stack lst => nth ((List.length lst)-i) lst ns
-    | no_stacks => 
-      match t_h loc with tuple lst => nth i lst ns end
+  match h with (s_h1,s_h2,t_h) =>
+    match stk_heap_app s_h1 loc,
+      stk_heap_app s_h2 loc,t_h loc with
+    | stack lst,no_stacks,tuple [] =>
+      nth ((List.length lst)-i) lst ns
+    | no_stacks,stack lst,tuple [] =>
+      nth ((List.length lst)-i) lst ns
+    | no_stacks,no_stacks,tuple lst => nth i lst ns
+    | _,_,_ => ns
     end
   end.
 (* --------------------------------------------
@@ -242,108 +275,161 @@ Inductive step (P:program) : (heap * reg_file) ->
 (heap * reg_file) -> Prop :=
   | S_add : forall (H:heap) (R:reg_file) (l:code_location)
     (reg:register) (o:operand) (w1 w2: nat),
-    reg_app R ip = l -> fetch_instr l P = add reg o
-    -> reg_app R reg = int_w w1 -> operand_value o R = int_w w2 ->
+    reg_app R ip = l -> fetch_instr l P = add reg o ->
+    reg_app R reg = int_w w1 -> operand_value o R = int_w w2 ->
     step P (H,R)
       (H, ip !->r next_cloc l; reg !->r w1+w2 ; R)
-  | S_mkstk : forall (H:heap) (R:reg_file) (l:code_location)
-    (reg:register) (L:heap_loc),
+  | S_mkstk : forall (H_stk H_cont:stack_heap) (H_tup:tuple_heap)
+      (R:reg_file) (l:code_location) (reg:register) (L:heap_loc),
     reg_app R ip = l -> fetch_instr l P = mkstk reg
-    -> heap_app H L = inr (tuple nil) ->
-    step P (H,R)
-      (L !->h inl (stack nil) ; H,
+    -> fresh (H_stk,H_cont,H_tup) L = true ->
+    step P (H_stk,H_cont,H_tup,R)
+      ((L,stack nil) :: H_stk,H_cont,H_tup,
       ip !->r next_cloc l; reg !->r hloc L 0; R)
-  | S_salloc : forall (H:heap) (R:reg_file) (l:code_location)
-              (n j:nat) (lsp:heap_loc) (lst:list word),
+  | S_salloc : forall (H_stk H_stk' H_cont:stack_heap)
+      (H_tup:tuple_heap) (R:reg_file) (l:code_location) (n j:nat)
+      (lsp:heap_loc) (lst:list word),
     reg_app R ip = l -> fetch_instr l P = salloc n
-    -> reg_app R sp = hloc lsp j -> heap_app H lsp = inl (stack lst)
+    -> reg_app R sp = hloc lsp j
+    -> H_stk = (lsp, stack lst) :: H_stk'
     -> List.length lst = j ->
-    step P (H,R)
-      (lsp !->h inl (stack (n_cons n ns lst)); H ,
+    step P (H_stk,H_cont,H_tup,R)
+      ((lsp,stack (n_cons n ns lst)) :: H_stk',H_cont,H_tup,
       ip !->r next_cloc l; sp !->r  hloc lsp (j+n); R)
-  | S_push : forall (H:heap) (R:reg_file) (l:code_location)
-           (o:operand) (j:nat) (lsp:heap_loc) (lst:list word),
+  | S_push : forall (H_stk H_stk' H_cont:stack_heap)
+      (H_tup:tuple_heap) (R:reg_file) (l:code_location)
+      (o:operand) (j:nat) (lsp:heap_loc) (lst:list word),
     reg_app R ip = l -> fetch_instr l P = push o
-    -> reg_app R sp = hloc lsp j -> heap_app H lsp = inl (stack lst)
+    -> reg_app R sp = hloc lsp j
+    -> H_stk = (lsp, stack lst) :: H_stk'
     -> List.length lst = j ->
-    step P (H,R)
-      (lsp !->h inl (stack (cons (operand_value o R) lst)); H ,
+    step P (H_stk,H_cont,H_tup,R)
+      ((lsp,stack (cons (operand_value o R) lst)) :: H_stk',
+      H_cont, H_tup,
       ip !->r next_cloc l; sp !->r hloc lsp (1+j); R)
-  | S_sfree : forall (H:heap) (R:reg_file) (l:code_location)
-            (j n:nat) (reg:register) (lsp:heap_loc) (lst:list word),
+  | S_sfree : forall (H_stk H_stk' H_cont:stack_heap)
+      (H_tup:tuple_heap) (R:reg_file) (l:code_location)
+      (j n:nat) (lsp:heap_loc) (lst:list word),
     reg_app R ip = l -> fetch_instr l P = sfree n
-    -> reg_app R reg = hloc lsp j -> heap_app H lsp = inl (stack lst)
+    -> reg_app R sp = hloc lsp j
+    -> H_stk = (lsp, stack lst) :: H_stk'
     -> j >= n -> List.length lst = j ->
-    step P (H,R)
-      (lsp !->h inl (stack (cdr_nth n lst)); H,
+    step P (H_stk,H_cont,H_tup,R)
+      ((lsp,stack (cdr_nth n lst)) :: H_stk',H_cont,H_tup,
       ip !->r next_cloc l; sp !->r  hloc lsp (j-n); R)
-  | S_pop : forall (H:heap) (R:reg_file) (l:code_location)
-          (j:nat) (reg:register) (lsp:heap_loc) (lst:list word),
+  | S_pop : forall (H_stk H_stk' H_cont:stack_heap)
+      (H_tup:tuple_heap) (R:reg_file) (l:code_location)
+      (j:nat) (reg:register) (lsp:heap_loc) (lst:list word),
     reg_app R ip = l -> fetch_instr l P = pop reg
-    -> reg_app R sp = hloc lsp j -> heap_app H lsp = inl (stack lst)
+    -> reg_app R sp = hloc lsp j
+    -> H_stk = (lsp, stack lst) :: H_stk'
     -> j > 0 -> List.length lst = j ->
-    step P (H,R)
-      (lsp !->h inl (stack (cdr_nth 1 lst)); H,
+    step P (H_stk,H_cont,H_tup,R)
+      ((lsp,stack (cdr_nth 1 lst)) :: H_stk',H_cont,H_tup,
       ip !->r next_cloc l; reg !->r (List.hd ns lst);
       sp !->r  hloc lsp (j-1); R)
-  | S_malloc : forall (H:heap) (R:reg_file) (l:code_location)
-    (i d:nat) (L:heap_loc),
+  | S_malloc : forall (H_stks:stack_heap * stack_heap) (H_tup:tuple_heap)
+    (R:reg_file) (l:code_location) (i d:nat) (L:heap_loc),
     reg_app R ip = l -> fetch_instr l P = malloc d i
-    -> heap_app H L = inr (tuple nil) ->
-    step P (H,R)
-      (L !->h inr (tuple (n_cons i ns nil)) ; H,
+    -> fresh (H_stks,H_tup) L = true ->
+    step P (H_stks,H_tup,R)
+      (H_stks,L !->t tuple (n_cons i ns nil) ; H_tup,
       ip !->r next_cloc l ; d !->r hloc L 0 ;R)
   | S_mov : forall (H:heap) (R:reg_file) (l:code_location)
     (d:nat) (o:operand),
     reg_app R ip = l -> fetch_instr l P = mov d o ->
     step P (H,R)
       (H, ip !->r next_cloc l; d !->r (operand_value o R); R)
-  | S_mov_sp : forall (H:heap) (R:reg_file) (l:code_location)
-             (o:operand) (L:heap_loc) (lst:list word) (j k:nat),
+  | S_mov_sp_raise : forall (H_stk H_stk_hd H_stk' H_cont:stack_heap)
+      (H_tup:tuple_heap) (R:reg_file) (l:code_location)
+      (o:operand) (L:heap_loc) (lst:list word) (j k:nat),
     reg_app R ip = l -> fetch_instr l P = mov sp o
-    -> operand_value o R = hloc L j -> heap_app H L = inl (stack lst)
+    -> operand_value o R = hloc L j
+    -> H_stk = H_stk_hd ++ (L, stack lst) :: H_stk'
     -> List.length lst = k -> j <= k ->
-    step P (H,R)
-      (L !->h inl (stack (cdr_nth (k-j) lst)); H,
+    step P (H_stk,H_cont,H_tup,R)
+      ((L,stack (cdr_nth (k-j) lst)) :: H_stk',
+      (rev H_stk_hd) ++ H_cont, H_tup,
       ip !->r next_cloc l; sp !->r hloc L j ; R)
-  | S_load : forall (H:heap) (R:reg_file) (l:code_location)
-    (L:heap_loc) (d s j:nat),
-    reg_app R ip = l -> fetch_instr l P = load d s j
+  | S_mov_sp_resume : forall (H_stk H_cont_hd H_cont' H_cont:stack_heap)
+      (H_tup:tuple_heap) (R:reg_file) (l:code_location)
+      (o:operand) (L:heap_loc) (lst:list word) (j k:nat),
+    reg_app R ip = l -> fetch_instr l P = mov sp o
+    -> operand_value o R = hloc L j
+    -> H_cont = H_cont_hd ++ (L, stack lst) :: H_cont'
+    -> List.length lst = k -> j <= k ->
+    step P (H_stk,H_cont,H_tup,R)
+      ((L,stack (cdr_nth (k-j) lst)) :: (rev H_cont_hd) ++ H_stk,
+      H_cont', H_tup,
+      ip !->r next_cloc l; sp !->r hloc L j ; R)
+  | S_mov_sp_lvhdl : forall (H_stk H_stk_hd H_stk' H_cont:stack_heap)
+      (H_tup:tuple_heap) (R:reg_file) (l:code_location)
+      (o:operand) (L:heap_loc) (lst:list word) (j k:nat),
+    reg_app R ip = l -> fetch_instr l P = mov sp o
+    -> operand_value o R = hloc L j
+    -> H_stk = H_stk_hd ++ (L, stack lst) :: H_stk'
+    -> List.length lst = k -> j <= k ->
+    step P (H_stk,H_cont,H_tup,R)
+      ((L,stack (cdr_nth (k-j) lst)) :: H_stk',
+      H_cont, H_tup,
+      ip !->r next_cloc l; sp !->r hloc L j ; R)
+  | S_load_stk : forall (H_stk H_cont:stack_heap)
+      (H_tup:tuple_heap) (R:reg_file) (l:code_location)
+    (L:heap_loc) (s:register) (d off i:nat) lst (sign:bool),
+    (* true means addition and false subtraction *)
+    reg_app R ip = l -> fetch_instr l P = load d s sign off
+    -> reg_app R s = hloc L i ->
+    stk_heap_app H_stk L = stack lst \/
+    stk_heap_app H_cont L = stack lst ->
+    step P (H_stk,H_cont,H_tup,R)
+      (H_stk,H_cont,H_tup, ip !->r next_cloc l;
+      d !->r nth
+        (match sign, List.length lst with
+        | true, len=> len - i - off
+        | false, len => len - i + off end)
+        lst ns; R)
+  | S_load_tup : forall (H_stk H_cont:stack_heap)
+      (H_tup:tuple_heap) (R:reg_file) (l:code_location)
+    (L:heap_loc) (s:register) (d off:nat) lst,
+    reg_app R ip = l -> fetch_instr l P = load d s true off
     -> reg_app R s = hloc L 0 ->
-    step P (H,R)
-      (H, ip !->r next_cloc l; d !->r fetch_heap L j H ; R)
-  | S_store : forall (H:heap) (R:reg_file) (l:code_location)
+    H_tup L = tuple lst ->
+    step P (H_stk,H_cont,H_tup,R)
+      (H_stk,H_cont,H_tup, ip !->r next_cloc l;
+      d !->r nth off lst ns; R)
+  | S_store : forall (H_stks:stack_heap * stack_heap) (H_tup:tuple_heap)
+    (R:reg_file) (l:code_location)
     (L:heap_loc) (d j:nat) (o:operand) (lst:list word),
     reg_app R ip = l -> fetch_instr l P = store d j o
-    -> reg_app R d = hloc L 0 -> heap_app H L = inr (tuple lst) -> j < List.length lst ->
-    step P (H,R)
-      (L !->h inr (tuple (update_nth j lst (operand_value o R))); H,
+    -> reg_app R d = hloc L 0
+    -> H_tup L = tuple lst
+    -> j < List.length lst ->
+    step P (H_stks,H_tup,R)
+      (H_stks,L !->t tuple (update_nth j lst (operand_value o R)); H_tup,
       ip !->r next_cloc l; R)
-  | S_call : forall (H:heap) (R:reg_file) (l l':code_location)
-    (lsp:heap_loc) (j:nat) (o:operand) (lst:list word),
+  | S_call : forall (H_stk H_stk' H_cont:stack_heap)
+      (H_tup:tuple_heap) (R:reg_file) (l l_dst:code_location)
+      (lsp:heap_loc) (j:nat) (o:operand) (lst:list word),
     reg_app R ip = l -> fetch_instr l P = call o
-    -> reg_app R sp = hloc lsp j -> heap_app H lsp = inl (stack lst)
-    -> List.length lst = j -> operand_value o R = l' ->
-    step P (H,R)
-      (lsp !->h inl (stack (cons (loc_w(next_cloc l)) lst)) ; H,
-      ip !->r l' ; R)
+    -> reg_app R sp = hloc lsp j -> H_stk = (lsp,stack lst) :: H_stk'
+    -> List.length lst = j -> operand_value o R = l_dst ->
+    step P (H_stk,H_cont,H_tup,R)
+      ((lsp,stack ((loc_w(next_cloc l)) :: lst)) :: H_stk',H_cont,H_tup,
+      ip !->r l_dst ; R)
   | S_jmp : forall (H:heap) (R:reg_file) (l l':code_location)
     (o:operand),
     reg_app R ip = l -> fetch_instr l P = jmp o
     -> operand_value o R = l' ->
     step P (H,R) (H, ip !->r l' ; R)
-  | S_ret : forall (H:heap) (R:reg_file) (l l':code_location)
+  | S_ret : forall (H_stk H_stk' H_cont:stack_heap)
+      (H_tup:tuple_heap) (R:reg_file) (l l':code_location)
     (lst:list word) (j:nat) (lsp:heap_loc),
     reg_app R ip = l -> fetch_instr l P = ret
     -> reg_app R sp = hloc lsp j ->
-    heap_app H lsp = inl (stack (cons (loc_w l') lst))
+    H_stk = (lsp,stack ((loc_w l') :: lst)) :: H_stk'
     -> List.length lst = j-1 ->
-    step P (H,R)
-      (lsp !->h inl (stack lst) ; H, ip !->r l' ; R)
-  | S_halt : forall (H:heap) (R:reg_file) (l:code_location),
-    reg_app R ip = l -> fetch_instr l P = halt ->
-    step P (H,R) (H,R).
-
+    step P (H_stk,H_cont,H_tup,R)
+      ((lsp,stack lst)::H_stk',H_cont,H_tup, ip !->r l' ; R).
 (* Some properties and lemmas to be used later 
 Lemma reg_eqb_refl : forall a, reg_eqb a a = true.
 Proof with simpl;try reflexivity;auto.
@@ -466,3 +552,35 @@ Proof with automation.
 Qed.
 Lemma h_eqb_refl : forall (a:heap_loc), a = a -> h_eqb a a = true.
 Proof. intros. unfold h_eqb. destruct a. apply eqb_refl. Qed.
+(*
+raise abort's translation involves mov sp r1
+label_handle involves mkstk sp, and mov sp r2 in the end.
+  how handle works: make a new stack temporarily, call the function
+  then ignore the new stack and go back to previous stack
+
+label_raise
+  sp now gets the location given by argument v1, translated to r1
+  we then call the handler
+label_resume
+  similar, we also put content in r1 to sp
+
+normally, sp points to top of first stack. When raising, sp points
+to some middle stack, when resuming, sp go back to some stack
+So we can view H_stack as two chuncks, 1 representing K of lexi,
+the other representing heap of continuations.
+*)
+(*
+change sfree from r to sp in premise. Wrong register
+
+load: used in 
+  translating variables, 
+  getting value/pi (load r1 r1 i): load from tuple,
+    r1 always have offset 0, no need to special consider
+  raise: load from stack, counting from bottom, also
+    always offset 0
+      nonono, these are also counting from top of stack
+  raise general:
+  resume:
+I do also notice though that since stack pointer counts from the base, but variable/de brujin index counts from the top of stack, the translated code should be 
+raising handler has wrong offsets
+*)
