SimProof.v
@@ -31,19 +31,19 @@ Ltac automation :=
 Theorem cond1 : forall C1 C2 M1 M2 main_lab init_lab,
   code_trans C1 = C2 ->
   init_L (c_lab init_lab) (letrec C1 (bind (app (c_lab main_lab) [])
-    (bind (exit (ind_val 1)) (val_term L.ns)))) M1
+    (bind (exit (ind_val 1)) (val_term 0)))) M1
   -> init_S (cloc_str init_lab) (cloc_str main_lab) C2 M2 -> LS_rel M1 M2.
 Proof with automation.
   intros. destruct M1 as [[[[LC LH] LK] LE] Lt], M2 as [[SC SH] SR].
   inversion H1... inversion H0...
   apply rel_LS with (len:=0) (Clab:=init_lab) (lst:=[])
     (SIlst:=[mov 0 (cloc main_lab 0); call 0;
-    push (reg_o 1); load 1 sp 1; halt])
+    push (reg_o 1); load 1 sp false 1; halt])
     (Slsp:=hloc L_stack 0)...
   - destruct L_stack as [L_stack_str].
     apply rel_context with (Ks:=[]) (Flst:=[]) (E:=[])
       (s:=[]) (s':=[]) (s_out:=[]) (L_out:=L_stack_str) 
-      (L_0:=L_stack_str) (newL_out:=hloc L_stack_str 0)
+      (L_0:=L_stack_str)
       (H_stack:=sh_empty)...
   - unfold S.c_update,S.c_eqb. rewrite eqb_refl...
 Qed.
@@ -69,6 +69,9 @@ Proof with automation.
   - apply app_cons_not_nil.
   - destruct a...
 Qed.
+
+
+
 Theorem cond3 : forall LC SC H1 K1 E1 t1 R2 H2 H1' K1' E1' t1',
   LS_rel (LC, H1, K1, E1, t1)
     (SC, H2, R2) ->
@@ -80,21 +83,21 @@ Theorem cond3 : forall LC SC H1 K1 E1 t1 R2 H2 H1' K1' E1' t1',
 Proof with automation.
   intros. inversion H... inversion H12...
   inversion H0;automation;
-  remember (map val_env_trans E1 ++ s_out) as cur_stk_val;
+  remember (map run_cst_trans E1 ++ s_out) as cur_stk_val;
   remember (cloc Clab (List.length lst)) as l;
-  remember (L_out !->s stack cur_stk_val; H_stack) as cur_stkh.
+  remember ((L_out,stack cur_stk_val)::H_stack) as cur_stkh.
   (* 14 stepping rules, prove the multi and rel for each *)
-  - exists
-      (L_out !->h inl (stack ((int_w (i1+i2)) :: cur_stk_val));
-        (cur_stkh,SH_heap)),
+  - (* x = v1 + v2 *) exists
+      ((L_out,stack ((int_w (i1+i2)) :: cur_stk_val))
+        :: H_stack,SH_cont,SH_tup),
       ([(ip,loc_w (incr_cloc 4 l));(sp,loc_w (hloc L_out
         (1+(List.length cur_stk_val))));
         (nat_reg 1,int_w (i1+i2));(nat_reg 2,int_w i2);
         (nat_reg 3,o3);(nat_reg 4,o4);(nat_reg 5,o5);
         (nat_reg 6,o6)]). split.
-    (* manually stepping translated salt code for L_add*)
+    (* stepping translated salt code for addition *)
     + apply multi_step with (*y is 1 step after current*)
-      (y:=((cur_stkh, SH_heap),
+      (y:=((cur_stkh,SH_cont,SH_tup),
         [(ip,loc_w (next_cloc l));(sp,loc_w (hloc L_out
         (List.length cur_stk_val)));(nat_reg 1,int_w i1);
         (nat_reg 2,o2);(nat_reg 3,o3);
@@ -104,9 +107,9 @@ Proof with automation.
           (List.length cur_stk_val)));
           (nat_reg 1,o1);(nat_reg 2,o2);(nat_reg 3,o3);
           (nat_reg 4,o4);(nat_reg 5,o5);(nat_reg 6,o6)])
-        (H:=(cur_stkh,SH_heap)) (P:=SC)... inversion H10.
+        (H:=(cur_stkh,SH_cont,SH_tup)) (P:=SC)... inversion H10.
         simpl. rewrite H15... cbn. apply nth_middle. }
-      apply multi_step with (y:=((cur_stkh, SH_heap),
+      apply multi_step with (y:=((cur_stkh, SH_cont,SH_tup),
       [(ip,loc_w (incr_cloc 2 l));(sp,loc_w (hloc L_out
       (List.length cur_stk_val)));(nat_reg 1,int_w i1);
       (nat_reg 2,int_w i2);(nat_reg 3,o3);
@@ -116,7 +119,7 @@ Proof with automation.
           (sp,loc_w (hloc L_out (List.length cur_stk_val)));
           (nat_reg 1,int_w i1);(nat_reg 2,o2);(nat_reg 3,o3);
           (nat_reg 4,o4);(nat_reg 5,o5);(nat_reg 6,o6)])
-        (H:=(cur_stkh,SH_heap)) (P:=SC)... inversion H10.
+        (H:=(cur_stkh,SH_cont,SH_tup)) (P:=SC)... inversion H10.
         simpl. rewrite H15... rewrite <- last_length with (a:=mov 1 i1).
         cbn. assert (List_swp:forall lst', lst ++
         (mov 1 i1::mov 2 i2::lst')=
@@ -126,16 +129,16 @@ Proof with automation.
           (a:=mov 2 i2)(l:=lst++[mov 1 i1])
           (l':=tl (tl(LS.func_term_trans (Datatypes.length E1)
             (L.bind (L.add 
-            (L.const_val (L.nat_const i1))
-            (L.const_val (L.nat_const i2))) t1')))). }
-      apply multi_step with (y:=((cur_stkh, SH_heap),
+            (L.st_cst_val i1)
+            (L.st_cst_val i2)) t1')))). }
+      apply multi_step with (y:=((cur_stkh,SH_cont,SH_tup),
       [(ip,loc_w (incr_cloc 3 l));(sp,loc_w (hloc L_out
       (List.length cur_stk_val)));(nat_reg 1,int_w (i1+i2));
       (nat_reg 2,int_w i2);(nat_reg 3,o3);
       (nat_reg 4,o4);(nat_reg 5,o5);(nat_reg 6,o6)])).
       { apply S_add with (w1:=i1) (w2:=i2) (reg:=nat_reg 1)
         (o:=reg_o (nat_reg 2)) (l:=incr_cloc 2 l)
-        (H:=(cur_stkh,SH_heap)) (R:=[(ip,loc_w (incr_cloc 2 l));
+        (H:=(cur_stkh,SH_cont,SH_tup)) (R:=[(ip,loc_w (incr_cloc 2 l));
           (sp,loc_w (hloc L_out (List.length cur_stk_val)));
           (nat_reg 1,int_w i1);(nat_reg 2,int_w i2);
           (nat_reg 3,o3);(nat_reg 4,o4);(nat_reg 5,o5);
@@ -146,18 +149,17 @@ Proof with automation.
           rewrite Temp.
           apply app_nth2_plus with (n:=2) (l:=lst). }
       constructor.
-      { apply S_push with (l:=incr_cloc 3 l) (lsp:=L_out)
-        (o:=reg_o (nat_reg 1)) (lst:=cur_stk_val)
-        (j:=List.length cur_stk_val) (H:=(cur_stkh, SH_heap))
-        (R:=[(ip,loc_w (incr_cloc 3 l));(sp,loc_w (hloc L_out
-          (List.length cur_stk_val)));(nat_reg 1,int_w (i1+i2));
-          (nat_reg 2,int_w i2);(nat_reg 3,o3);(nat_reg 4,o4);
-          (nat_reg 5,o5);(nat_reg 6,o6)]);automation;simpl.
-        - rewrite H15. assert (Temp:forall n, S (S (S n)) = n + 3).
-          { intros. rewrite PeanoNat.Nat.add_comm... } inversion H10...
-          rewrite Temp. apply app_nth2_plus with (n:=3) (l:=lst).
-        - simpl. destruct L_out as [L_out_str]. unfold sh_update,h_eqb.
-          rewrite eqb_refl... }
+      apply S_push with (l:=incr_cloc 3 l) (lsp:=L_out)
+      (o:=reg_o (nat_reg 1)) (lst:=cur_stk_val)
+      (j:=List.length cur_stk_val) (H_stk:=cur_stkh) 
+      (H_cont:=SH_cont) (H_tup:=SH_tup)
+      (R:=[(ip,loc_w (incr_cloc 3 l));(sp,loc_w (hloc L_out
+        (List.length cur_stk_val)));(nat_reg 1,int_w (i1+i2));
+        (nat_reg 2,int_w i2);(nat_reg 3,o3);(nat_reg 4,o4);
+        (nat_reg 5,o5);(nat_reg 6,o6)]);automation;simpl.
+      rewrite H15. assert (Temp:forall n, S (S (S n)) = n + 3).
+      { intros. rewrite PeanoNat.Nat.add_comm... } inversion H10...
+      rewrite Temp. apply app_nth2_plus with (n:=3) (l:=lst).
     (* prove LS_rel for L_add *)
     + unfold h_update,incr_cloc,next_cloc... apply rel_LS with
       (lst:=lst ++ firstn 4 SIlst)
@@ -165,23 +167,107 @@ Proof with automation.
       * cbn. pose proof term_trans_not_nil as NN. specialize NN with
         (tm:=t1'). destruct (RelConfig.LS.term_trans t1')as []eqn:?...
         rewrite <- Heql. rewrite <- PeanoNat.Nat.add_succ_comm.
-        apply rel_tm with (E:=L.nat_const (i1 + i2) :: E1) (t:=t1').
+        apply rel_tm with (E:=L.st_run_cst (i1 + i2) :: E1) (t:=t1').
       * apply rel_context with (s:=s) (s_out:=s_out)
-        (L_0:=L_0)... apply rel_hdl_general. inversion H7...
-        -- 
+        (L_0:=L_0)...
+      * rewrite H15. cbn. assert (AssocIns: forall (x1:instr) x2 x3 x4 tl,
+          [x1;x2;x3;x4] ++ tl = x1::x2::x3::x4::tl). { intros... }
+        rewrite <- AssocIns,app_assoc_reverse...
+      * rewrite app_length. rewrite PeanoNat.Nat.add_comm...
+  - (* x = v *) exists
+      ((L_out,stack ((val_direct_trans v cur_stk_val) :: cur_stk_val))
+        :: H_stack,SH_cont,SH_tup),
+      ([(ip,loc_w (incr_cloc 2 l));(sp,loc_w (hloc L_out
+        (1+(List.length cur_stk_val))));
+        (nat_reg 1,val_direct_trans v cur_stk_val);(nat_reg 2,o2);
+        (nat_reg 3,o3);(nat_reg 4,o4);(nat_reg 5,o5);
+        (nat_reg 6,o6)]). split.
+    + (* stepping translated salt code for single value *)
+      apply multi_step with (*y is 1 step after current*)
+      (y:=((cur_stkh,SH_cont,SH_tup),
+        [(ip,loc_w (next_cloc l));(sp,loc_w (hloc L_out
+        (List.length cur_stk_val)));(nat_reg 1,
+          val_direct_trans v cur_stk_val);
+        (nat_reg 2,o2);(nat_reg 3,o3);(nat_reg 4,o4);
+        (nat_reg 5,o5);(nat_reg 6,o6)])).
+      { destruct v as [cst|[ind]].
+        - apply S_mov with (d:=1)
+        (o:=val_direct_trans (st_cst_val cst) cur_stk_val)
+        (l:=l) (R:=[(ip,loc_w l);(sp,loc_w (hloc L_out
+          (List.length cur_stk_val)));
+          (nat_reg 1,o1);(nat_reg 2,o2);(nat_reg 3,o3);
+          (nat_reg 4,o4);(nat_reg 5,o5);(nat_reg 6,o6)])
+        (H:=(cur_stkh,SH_cont,SH_tup)) (P:=SC)...
+        inversion H10... cbn. rewrite H15...
+        apply nth_middle.
+        - pose proof S_load_stk as Ins. specialize Ins with
+          (d:=1) (s:=sp) (off:=ind)
+          (L:=L_out) (H_stk:=cur_stkh) (H_cont:=SH_cont)
+          (H_tup:=SH_tup) (sign:=false)
+          (lst:=cur_stk_val) (i:=List.length cur_stk_val)
+          (R:=[(ip,loc_w l);(sp,loc_w (hloc L_out
+          (List.length cur_stk_val)));
+          (nat_reg 1,o1);(nat_reg 2,o2);(nat_reg 3,o3);
+          (nat_reg 4,o4);(nat_reg 5,o5);(nat_reg 6,o6)])
+          (l:=l) (P:=SC). rewrite PeanoNat.Nat.sub_diag in Ins.
+          apply Ins;automation;cbn.
+          + inversion H10. rewrite H15... apply nth_middle.
+          + rewrite h_eqb_refl... }
+      constructor.
+      apply S_push with (H_stk:=cur_stkh) (H_cont:=SH_cont)
+      (H_tup:=SH_tup) (l:=next_cloc l) (o:=reg_o 1) (lsp:=L_out)
+      (lst:=cur_stk_val) (j:=List.length cur_stk_val)
+      (R:=[(ip,loc_w (next_cloc l));
+      (sp,loc_w(hloc L_out (Datatypes.length cur_stk_val)));
+      (nat_reg 1,val_direct_trans v cur_stk_val);
+      (nat_reg 2,o2);(nat_reg 3,o3);
+      (nat_reg 4,o4);(nat_reg 5,o5);(nat_reg 6,o6)])...
+      cbn. rewrite H15. assert (Temp:forall n, S n = n + 1).
+      { intros. rewrite PeanoNat.Nat.add_comm... }
+      inversion H10... rewrite Temp.
+      apply app_nth2_plus with (n:=1) (l:=lst).
+    + (* prove LS_rel for x=v *)
+      rewrite Heql. apply rel_LS with (lst:=lst ++ 
+        firstn 2 SIlst) (SIlst:= tl (tl SIlst))...
+      * inversion H10. cbn. pose proof term_trans_not_nil as NN.
+        specialize NN with (tm:=t1'). destruct
+        (RelConfig.LS.term_trans t1')as []eqn:?... rewrite <- Heql.
+        rewrite <- PeanoNat.Nat.add_succ_comm.
+        apply rel_tm with (E:=L.var_deref E1 v :: E1) (t:=t1').
+      * apply rel_context with (s:=s) (s_out:=s_out)
+        (L_0:=L_0)... destruct v as [cst|[ind]];cbn...
+        rewrite <- map_nth with (d:=L.ns). rewrite app_nth1...
+(* need to guarantee that in programs entered by user,
+   de brujin indices aren't out of range *)
+      * rewrite H15. cbn. assert (AssocIns: forall (x1:instr) x2 x3 x4 tl,
+          [x1;x2;x3;x4] ++ tl = x1::x2::x3::x4::tl). { intros... }
+        rewrite <- AssocIns,app_assoc_reverse...
+      * rewrite app_length. rewrite PeanoNat.Nat.add_comm...
+
+Inductive LS_rel :
+  (L.code * L.heap * L.eval_context * L.local_env * L.term)
+  -> (S.program * S.heap * reg_file) -> Prop :=
+  rel_LS : forall len lst SIlst
+    LC LH LK LE Lt SC o1 o2 o3 o4 o5 o6
+    (SH_stack:stack_heap) (SH_cont:stack_heap)
+    (SH_tup:tuple_heap)
+    (Slsp:heap_location) Clab,
+    LS_rel_ins (LE,Lt) (ins_seq SIlst) ->
+    LS_rel_context (LK,LE) (SH_stack,Slsp) ->
+    LS_rel_heap LH (SH_cont,SH_tup) -> LS_rel_code LC SC ->
+    SC Clab = ins_seq (lst ++ SIlst) -> List.length lst = len ->
+    LS_rel (LC, LH, LK, LE, Lt)
+      (SC, (SH_stack,SH_cont,SH_tup),
+        [(ip,loc_w (cloc Clab len));(sp,loc_w Slsp);(nat_reg 1,o1);
+        (nat_reg 2,o2);(nat_reg 3,o3);(nat_reg 4,o4);
+        (nat_reg 5,o5);(nat_reg 6,o6)]).
+
 (*other things
 0. changes in lexi heaps e.g. assignment
 1. handler related stuff
 2. relating data heap
 3. relating hdl-led-ctx*)
 
-only change:
-(x !->e L.nat_const (i1 + i2); E1)%L_scope =
-      E1'
-SI = (ins_seq (LS.func_term_trans (map fst E) t))
-SC Clab = concat_ins_seq lst SI
-
-LS_rel_context (LK,E) ((SH_stack,th_empty),Slsp)
 Qed.
 (*
 0. redefine salt's opsem s.t. register files only have finite registrers
@@ -196,6 +282,7 @@ Qed.
 (*
 All changes made
 *)
+
 
 
 
